basic counter module should work

examples/counter/extraction/CounterConcordiumWasm.v
@@ -2,39 +2,66 @@ Unset Universe Checking.
 From ConCert.Examples.Counter Require Counter.
 From ConCert.Extraction Require Import Common.
 From ConCert.Extraction Require Import ConcordiumExtract.
-From ConCert.Extraction Require Import SpecializeChainBase.
-From RustExtraction Require Import RustExtract.
-From Coq Require Import Bool.
-From Coq Require Import String.
+From Coq Require Import List Uint63 ZArith Bool String.
 From MetaCoq.Template Require Import All.
 
-Open Scope string.
+From ConCert.Execution Require Import Blockchain BoundedN.
+Import ssreflect.
 
-Definition COUNTER_MODULE : ConcordiumMod _ _ :=
-  {| concmd_contract_name := "counter"%bs;
-     concmd_init := @ConCert.Examples.Counter.Counter.counter_init;
-     concmd_receive := @ConCert.Examples.Counter.Counter.counter_receive;
-     concmd_extra := []; |}.
+(* Extraction of the counter contract to Wasm (for Concordium) via CertiCoq-Wasm.
 
-(* NOTE: it is important to declare a printing config, otherwise MetaCoq evaluation tries to normalize a term with an unresolved instance and runs out of memory. *)
-#[local]
-Instance RustConfig : RustPrintConfig :=
-    {| term_box_symbol := "()";
-       type_box_symbol := "()";
-       any_type_symbol := "()";
-       print_full_names := false |}.
-(*
-Redirect "../extraction/tests/extracted-code/concordium-extract/counter.rs"
-MetaCoq Run (concordium_extraction
-               COUNTER_MODULE
-               (ConcordiumRemap.build_remaps
-                  (ConcordiumRemap.remap_Z_arith ++ ConcordiumRemap.remap_blockchain_consts)
-                  []
-                  (ConcordiumRemap.remap_blockchain_inductives
-                     ++ ConcordiumRemap.remap_std_types))
-               (fun kn => eq_kername <%% bool_rec %%> kn
-                          || eq_kername <%% bool_rect %%> kn)).
+   concwmd_encode_state/concwmd_decode_state functions are tailored towards counter:
+   We use 8 bytes to store the value of the counter on the chain,
+   thus we convert the state to a Uint63.int.
+   CertiCoq-Wasm represents a Uint63.int as a Wasm i64 -> easy to get/set
+
+   To generalize for other contracts, the following is needed:
+   - include the Address as parameter for decode_state (not relevant for counter contract)
+   - need more bytes to store the state? a tuple/record of multiple Uint63.int would be suitable
+     E.g. CertiCoq-Wasm represents a tuple (Uint63.int, Uint63.int)
+     as a pointer p ---> [tag i64_0 i64_1], where the two i64s are placed directly next to each other.
+   - encode Chain (currently we pass a dummy value as the counter doesn't use it)
 *)
+
+
+Definition AddrSize : N := (2^8)%N.
+Lemma addr_serializable : Serializable.Serializable (BoundedN AddrSize).
+(* typeclasses eauto. *)
+Admitted.
+
+#[local]
+Instance LocalChainBase : ChainBase :=
+  {| Address := BoundedN AddrSize;
+     address_eqb := BoundedN.eqb;
+     address_eqb_spec := BoundedN.eqb_spec;
+     address_is_contract a := (AddrSize / 2 <=? BoundedN.to_N a)%N;
+     address_serializable := addr_serializable
+   |}.
+
+Record ConcordiumWasmMod (init_type receive_type : Type) (state : Type) :=
+{ concwmd_init : init_type;
+  concwmd_receive : receive_type;
+  concwmd_encode_state : state -> Uint63.int;
+  concwmd_decode_state : Uint63.int -> state
+}.
+
+Definition zero : BoundedN AddrSize. apply bounded with (n := 0%N). reflexivity.
+Defined.
+
+Definition encode_counter (s : Counter.State) : Uint63.int :=
+  match s with
+  | {| Counter.count := count; Counter.owner := _ |} => Uint63.of_Z count
+  end.
+
+Definition COUNTER_MODULE : ConcordiumWasmMod _ _ Counter.State :=
+  {| concwmd_init := @ConCert.Examples.Counter.Counter.counter_init LocalChainBase;
+     concwmd_receive := @ConCert.Examples.Counter.Counter.counter_receive LocalChainBase;
+     concwmd_encode_state := encode_counter;
+     concwmd_decode_state := fun p => Counter.build_state (Uint63.to_Z p) zero
+   |}.
+
+Check @COUNTER_MODULE.
+
 From CertiCoq.Plugin Require Import CertiCoq.
 CertiCoq Compile Wasm -debug COUNTER_MODULE.
 CertiCoq Show IR COUNTER_MODULE.
